Test/dafny0/NewtypesResolution.dfy
@@ -62,8 +62,8 @@ module Goodies {
     var ms := multiset{23.0, 50.0};
     assert forall rr :: 0.0 <= rr < 100.0  ==> ms[rr] == ms[rr];
 
-    var truncated := r0.Trunc + x.Trunc;
-    var rounded := (r0 + 0.5).Trunc;
+    var floored := r0.Floor + x.Floor;
+    var rounded := (r0 + 0.5).Floor;
   }
 }
 
